examples/iterators/FindMaxMap.dfy
@@ -1,13 +1,16 @@
 include "../../src/linear/adt/List.dfy"
 include "../../src/linear/impl/LinkedList.dfy"
 include "../../src/linear/impl/VectorImpl.dfy"
+include "../../src/Iterators_Utils.dfy"
 
-method FindMax(l: LinkedList) returns (max: ListIterator)
+function idMap(xs:seq<int>):map<int,int>
+{map i | 0<=i<=|xs| :: i}
+
+method FindMax(l: LinkedList) returns (max: ListIterator,ghost mit:map<int,int>)
   modifies l, l.Repr()
   requires l.Valid()
   requires l.Model() != []
   requires forall x | x in l.Repr() :: allocated(x)
-  
   ensures l.Valid()
   ensures l.Model() == old(l.Model())
   ensures fresh(max) && max in l.Iterators()
@@ -15,69 +18,21 @@ method FindMax(l: LinkedList) returns (max: ListIterator)
   ensures max.Parent() == l
   ensures max.HasNext()
   ensures forall x | x in l.Model() :: l.Model()[max.Index()] >= x
-
+  
   ensures l.Iterators() >= old(l.Iterators())
-  ensures forall it | it in old(l.Iterators()) && old(it.Valid()) ::
-    it.Valid() && it.Index() == old(it.Index())
+  ensures forall it | it in old(l.Iterators()) && old(it.Valid()) && old(it.Index()) in mit::it.Valid() && mit[old(it.Index())]==it.Index()
+  ensures mit==idMap(old(l.Model()))
+  ensures forall it | it in old(l.Iterators()) && old(it.Valid()):: old(it.Index()) in mit //domain
+  ensures forall i | i in mit :: mit[i]==i //range
 
   ensures forall x {:trigger x in l.Repr(), x in old(l.Repr())} | x in l.Repr() - old(l.Repr()) :: fresh(x)
   ensures forall x | x in l.Repr() - old(l.Repr()) :: fresh(x)
   ensures forall x | x in l.Repr() :: allocated(x)
-
+  
 {
-  max := l.Begin();
-  var it := l.Begin();
-  while it.HasNext()
-    decreases |l.Model()| - it.Index()
-    invariant l.Valid()
-    invariant l.Model() == old(l.Model())
-    invariant it.Valid()
-    invariant it in l.Iterators()
-    invariant fresh(max)
-    invariant max.Valid()
-    invariant max.Parent() == l
-    invariant max in l.Iterators()
-    invariant max != it
-    invariant max.HasNext()
-    invariant it.Index() <= |l.Model()|
-    invariant forall k | 0 <= k < it.Index() :: l.Model()[max.Index()] >= l.Model()[k]
-    
-    invariant l.Iterators() >= old(l.Iterators())
-    invariant forall it | it in old(l.Iterators()) && old(it.Valid()) ::
-      it.Valid() && it.Index() == old(it.Index())
+   mit:= map it | 0<=it<=|old(l.Model())|::it;
 
-    invariant forall x {:trigger x in l.Repr(), x in old(l.Repr())} | x in l.Repr() && x !in old(l.Repr()) :: fresh(x)
-    invariant forall x | x in l.Repr() :: allocated(x)
-    invariant forall x | x in old(l.Repr()) :: allocated(x)  
-  {
-    if it.Peek() > max.Peek() {
-      max := it.Copy();
-    }
-    var x := it.Next();
-  }
-}
 
-method FindMaxAL(l: ArrayList) returns (max: ListIterator)
-  modifies l, l.Repr()
-  requires l.Valid()
-  requires l.Model() != []
-  requires forall x | x in l.Repr() :: allocated(x)
-  ensures l.Valid()
-  ensures l.Model() == old(l.Model())
-  ensures fresh(max) && max in l.Iterators()
-  ensures max.Valid()
-  ensures max.Parent() == l
-  ensures max.HasNext()
-  ensures forall x | x in l.Model() :: l.Model()[max.Index()] >= x
-
-  ensures l.Iterators() >= old(l.Iterators())
-  ensures forall it | it in old(l.Iterators()) && old(it.Valid()) ::
-    it.Valid() && it.Index() == old(it.Index())
-
-  ensures forall x {:trigger x in l.Repr(), x in old(l.Repr())} | x in l.Repr() - old(l.Repr()) :: fresh(x)
-  ensures forall x | x in l.Repr() - old(l.Repr()) :: fresh(x)
-  ensures forall x | x in l.Repr() :: allocated(x)  
-{
   max := l.Begin();
   var it := l.Begin();
   while it.HasNext()
@@ -97,12 +52,76 @@ method FindMaxAL(l: ArrayList) returns (max: ListIterator)
     invariant forall k | 0 <= k < it.Index() :: l.Model()[max.Index()] >= l.Model()[k]
     
     invariant l.Iterators() >= old(l.Iterators())
-    invariant forall it | it in old(l.Iterators()) && old(it.Valid()) ::
-      it.Valid() && it.Index() == old(it.Index())
+    invariant forall it | it in old(l.Iterators()) && old(it.Valid()) && old(it.Index()) in mit::it.Valid() && mit[old(it.Index())]==it.Index();
 
     invariant forall x {:trigger x in l.Repr(), x in old(l.Repr())} | x in l.Repr() && x !in old(l.Repr()) :: fresh(x)
     invariant forall x | x in l.Repr() :: allocated(x)
-    invariant forall x | x in old(l.Repr()) :: allocated(x)  
+    invariant forall x | x in old(l.Repr()) :: allocated(x)
+    
+  {
+    if it.Peek() > max.Peek() {
+      max := it.Copy();
+    }
+    var x := it.Next();
+  }
+}
+
+
+method FindMaxAL(l: ArrayList) returns (max: ListIterator, ghost mit:map<int,int>)
+  modifies l, l.Repr()
+  requires l.Valid()
+  requires l.Model() != []
+  requires forall x | x in l.Repr() :: allocated(x)
+
+  ensures l.Valid()
+  ensures l.Model() == old(l.Model())
+  ensures fresh(max) && max in l.Iterators()
+  ensures max.Valid()
+  ensures max.Parent() == l
+  ensures max.HasNext()
+  ensures forall x | x in l.Model() :: l.Model()[max.Index()] >= x
+  
+
+  ensures l.Iterators() >= old(l.Iterators())
+  ensures forall it | it in old(l.Iterators()) && old(it.Valid()) && old(it.Index()) in mit::it.Valid() && mit[old(it.Index())]==it.Index()
+  ensures mit==buildMap((set it |it in old(l.Iterators()) && old(it.Valid())::old(it.Index())),identity)
+  ensures forall it | it in old(l.Iterators()) && old(it.Valid()):: old(it.Index()) in mit //domain
+  ensures forall i | i in mit :: mit[i]==identity(i) //range
+
+
+  ensures forall x {:trigger x in l.Repr(), x in old(l.Repr())} | x in l.Repr() - old(l.Repr()) :: fresh(x)
+  ensures forall x | x in l.Repr() - old(l.Repr()) :: fresh(x)
+  ensures forall x | x in l.Repr() :: allocated(x)  
+{
+    var setValid:=set it |it in old(l.Iterators()) && old(it.Valid())::old(it.Index());
+    mit:=buildMap(setValid,identity);
+
+
+  max := l.Begin();
+  var it := l.Begin();
+  while it.HasNext()
+    decreases |l.Model()| - it.Index()
+    invariant l.Valid()
+    invariant l.Model() == old(l.Model())
+    invariant it.Valid()
+    invariant it.Parent() == l
+    invariant it in l.Iterators()
+    invariant fresh(max)
+    invariant max.Valid()
+    invariant max.Parent() == l
+    invariant max in l.Iterators()
+    invariant max != it
+    invariant max.HasNext()
+    invariant it.Index() <= |l.Model()|
+    invariant forall k | 0 <= k < it.Index() :: l.Model()[max.Index()] >= l.Model()[k]
+    
+    invariant l.Iterators() >= old(l.Iterators())
+    invariant forall it | it in old(l.Iterators()) && old(it.Valid()) && old(it.Index()) in mit::it.Valid() && mit[old(it.Index())]==it.Index();
+
+    invariant forall x {:trigger x in l.Repr(), x in old(l.Repr())} | x in l.Repr() && x !in old(l.Repr()) :: fresh(x)
+    invariant forall x | x in l.Repr() :: allocated(x)
+    invariant forall x | x in old(l.Repr()) :: allocated(x)
+    
   {
     if it.Peek() > max.Peek() {
       max := it.Copy();
