examples/iterators/Misc.dfy
@@ -2,21 +2,70 @@ include "../../src/linear/adt/List.dfy"
 include "../../src/linear/impl/LinkedList.dfy"
 include "../../src/linear/impl/VectorImpl.dfy"
 
-method  IteratorExample1(l: List)
+method  allPositive(l: List) returns (b:bool)
   modifies l,l.Repr()
   requires l.Valid()
-  requires l.Model() != []
   requires forall x | x in l.Repr() :: allocated(x)
   ensures l.Valid()
   ensures l.Model() == old(l.Model())
+  ensures b== forall i| 0<=i<|old(l.Model())|::old(l.Model())[i]>=0
   ensures forall x {:trigger x in l.Repr(), x in old(l.Repr())} | x in l.Repr() && x !in old(l.Repr()) :: fresh(x)
   ensures fresh(l.Repr()-old(l.Repr()))
   ensures forall x | x in l.Repr() :: allocated(x)
 {
-  var it1 := l.Begin();
-  var x := it1.Next();
+ var elem,elem2;
+  var it1 := l.Begin(); 
+  var it2:=l.Begin(); if (it2.HasNext()) {elem2:=it2.Next();}
+  b:=true; 
+  while (it1.HasNext() && b )
+  decreases |l.Model()|-it1.Index()
+  invariant l.Valid() && it1.Valid() && it1.Parent()==l && it1 in l.Iterators()
+  invariant l.Model()==old(l.Model())
+  invariant 0<=it1.Index()<=|old(l.Model())|
+  invariant b==forall i | 0<=i<it1.Index():: old(l.Model())[i]>=0
+  invariant forall x {:trigger x in l.Repr(), x in old(l.Repr())} | x in l.Repr() && x !in old(l.Repr()) :: fresh(x)
+  invariant fresh(l.Repr()-old(l.Repr()))
+  invariant forall x | x in l.Repr() :: allocated(x)
+   { elem:=it1.Next(); 
+     b:=elem>=0;
+   }
 }
 
+
+method  allEqual(l: List) returns (b:bool)
+  modifies l,l.Repr()
+  requires l.Valid()
+  requires forall x | x in l.Repr() :: allocated(x)
+  ensures l.Valid()
+  ensures l.Model() == old(l.Model())
+  ensures b== forall i| 0<=i<|old(l.Model())|-1::old(l.Model())[i]==old(l.Model())[i+1]
+  ensures forall x {:trigger x in l.Repr(), x in old(l.Repr())} | x in l.Repr() && x !in old(l.Repr()) :: fresh(x)
+  ensures fresh(l.Repr()-old(l.Repr()))
+  ensures forall x | x in l.Repr() :: allocated(x)
+{
+ var elem,elem2;
+  var it1 := l.Begin(); 
+  var it2:=l.Begin(); if (it1.HasNext()) {elem:=it1.Next();}
+  b:=true; 
+  while (it1.HasNext() && b )
+  decreases |l.Model()|-it1.Index()
+  invariant l.Valid() && it1.Valid() && it1.Parent()==l && it1 in l.Iterators()
+  invariant it2.Valid() && it2.Parent()==l && it2 in l.Iterators()
+  invariant l.Model()==old(l.Model())
+  invariant 0<=it1.Index()<=|old(l.Model())| 
+  invariant it2.HasNext() ==> it2.Index()==it1.Index()-1
+  invariant it1.HasNext()==>it2.HasNext()
+  invariant b==forall i | 0<=i<it1.Index()-1:: old(l.Model())[i]==old(l.Model())[i+1]
+  invariant forall x {:trigger x in l.Repr(), x in old(l.Repr())} | x in l.Repr() && x !in old(l.Repr()) :: fresh(x)
+  invariant fresh(l.Repr()-old(l.Repr()))
+  invariant forall x | x in l.Repr() :: allocated(x)
+   {  
+     elem2:=it2.Next();
+     elem:=it1.Next();
+     b:=elem==elem2;
+   }
+   
+}
 method IteratorExample2(l: List)
   modifies l, l.Repr()
   requires l.Valid()
@@ -50,4 +99,21 @@ method  IteratorExample3(l: LinkedList)
   assert x == y;
   //assert !it1.Valid();  // we cannot prove nor disprove this assertion
   assert it2.Valid();
+}
+method  IteratorExample4(l: List)
+modifies l, l.Repr()
+  requires l.Valid()
+    requires forall x | x in l.Repr() :: allocated(x)
+  ensures l.Valid()
+  ensures forall x {:trigger x in l.Repr(), x in old(l.Repr())} | x in l.Repr() && x !in old(l.Repr()) :: fresh(x)
+  ensures fresh(l.Repr()-old(l.Repr()))
+  ensures forall x | x in l.Repr() :: allocated(x)
+
+{
+  var it1 := l.Begin();
+  var it2 := l.Begin();
+  it1:=l.Insert(it1,2);it1:=l.Insert(it1,2);
+  var b:=it1.HasNext();
+  if (it1.HasNext()) {it1:=l.Erase(it1);it1:=l.Insert(it1,4);}
+
 }
