examples/iterators/Quicksort.dfy
@@ -1,0 +1,334 @@
+include "../../src/linear/adt/List.dfy"
+include "../../src/linear/impl/LinkedList.dfy"
+
+predicate GSorted(xs:seq<int>,c:int,f:int)
+  { forall i,j | 0<=c<=i<=j<f<=|xs| :: xs[i]<=xs[j]}
+
+lemma  swapMultisetAux(xs:seq<int>,ys:seq<int>, i:int, j:int)
+requires 0<=i<|xs| && 0<=j<|ys| && i<=j && |xs|==|ys|
+requires forall z | 0<=z<|xs| && z!=i && z!=j :: xs[z]==ys[z]
+requires xs[i]==ys[j] && xs[j]==ys[i]
+ensures multiset(xs)==multiset(ys)
+{ 
+ if (i==j) {assert xs==ys;} 
+ else{  
+ calc=={
+   multiset(xs);{assert xs==xs[..i]+xs[i..j]+xs[j..];}
+   multiset(xs[..i]+xs[i..j]+xs[j..]);
+   {assert xs[i..j]==[xs[i]]+xs[i+1..j]; assert xs[j..] == [xs[j]]+xs[j+1..];}
+   multiset(xs[..i]+[xs[i]]+xs[i+1..j]+[xs[j]]+xs[j+1..]);
+   multiset(xs[..i])+multiset{xs[i]}+multiset(xs[i+1..j])+multiset{xs[j]}+multiset(xs[j+1..]);
+   multiset(xs[..i])+multiset{xs[i]}+multiset{xs[j]}+multiset(xs[i+1..j])+multiset(xs[j+1..]);
+   multiset(xs[..i])+multiset{xs[j]}+multiset{xs[i]}+multiset(xs[i+1..j])+multiset(xs[j+1..]);
+   multiset(xs[..i])+multiset{xs[j]}+multiset(xs[i+1..j])+multiset{xs[i]}+multiset(xs[j+1..]);
+   {assert xs[i]==ys[j] && xs[j]==ys[i]; 
+   assert xs[..i]==ys[..i];
+    assert xs[i+1..j]==ys[i+1..j];
+    assert xs[j+1..]==ys[j+1..];}
+   multiset(ys[..i])+multiset{ys[i]}+multiset(ys[i+1..j])+multiset{ys[j]}+multiset(ys[j+1..]);
+   {assert ys[i..j]==[ys[i]]+ys[i+1..j]; assert ys[j..] == [ys[j]]+ys[j+1..];}
+   multiset(ys[..i]+[ys[i]]+ys[i+1..j]+[ys[j]]+ys[j+1..]);
+      {assert [ys[i]]+ys[i+1..j]==ys[i..j]; assert [ys[j]]+ys[j+1..]==ys[j..];}
+   multiset(ys[..i]+ys[i..j]+ys[j..]);
+       {assert ys==ys[..i]+ys[i..j]+ys[j..];}
+   multiset(ys);
+}
+ }
+}
+
+lemma swapMultiset(xs:seq<int>,ys:seq<int>, i:int, j:int)
+requires 0<=i<|xs| && 0<=j<|ys| && |xs|==|ys|
+requires forall z | 0<=z<|xs| && z!=i && z!=j :: xs[z]==ys[z]
+requires xs[i]==ys[j] && xs[j]==ys[i]
+ensures multiset(xs)==multiset(ys)
+{
+  if (i<=j) {swapMultisetAux(xs,ys,i,j);}
+  else {swapMultisetAux(xs,ys,j,i);}
+
+
+}
+
+
+lemma multisetPreservesStrictSmaller (a:seq<int>, b:seq<int>, c:int, f:int, x:int)
+requires |a|==|b| && 0 <= c <= f + 1 <= |b| 
+requires (forall j :: c <= j <= f ==> a[j] < x)
+requires multiset(a[c..f+1]) == multiset(b[c..f+1])
+ensures (forall j :: c <= j <= f ==> b[j] < x)
+{if (c<=f){ 
+ forall j | c<=j<=f 
+   ensures b[j]<x
+  {   assert b[j] in b[c..f+1];
+      assert b[j] in multiset(a[c..f+1]);
+   }
+}
+}
+
+
+lemma multisetPreservesStrictGreater (a:seq<int>, b:seq<int>, c:int, f:int, x:int)
+requires |a|==|b| && 0 <= c <= f + 1 <= |b| 
+requires (forall j :: c <= j <= f ==> a[j] > x)
+requires multiset(a[c..f+1]) == multiset(b[c..f+1])
+ensures (forall j :: c <= j <= f ==> b[j] > x)
+{if (c<=f){ 
+ forall j | c<=j<=f 
+   ensures b[j]>x
+  {   assert b[j] in b[c..f+1];
+      assert b[j] in multiset(a[c..f+1]);
+   }
+}
+}
+
+lemma seqSplit(s:seq<int>, c:int, p:int, f:int)
+requires 0<=c<=p<=f+1<=|s|
+ensures multiset(s[c..f+1])==multiset(s[c..p])+multiset(s[p..f+1])
+{
+    calc=={
+  multiset(s[c..f+1]);
+  {assert s[c..f+1]==s[c..p]+s[p..f+1];}
+  multiset(s[c..p]+s[p..f+1]);
+  multiset(s[c..p])+multiset(s[p..f+1]);
+}
+}
+
+lemma subsecEq(xs:seq<int>,ys:seq<int>,c:int,f:int)
+requires 0<=c<=f<=|xs|==|ys|
+requires xs==ys
+ensures xs[c..f]==ys[c..f] && xs[c..]==ys[c..]&&xs[..f]==ys[..f]
+{}
+
+//Additional ghost results to know additional information 
+method swapG(l:LinkedList,p:ListIterator,q:ListIterator, ghost c:ListIterator, ghost n:int)
+modifies l, l.Repr(),p,q
+requires forall x | x in l.Repr() :: allocated(x)
+requires l.Valid() && p.Valid() && q.Valid()
+requires p in l.Iterators() && q in l.Iterators() 
+requires p.Parent()==l && q.Parent()==l
+requires p.HasNext() && q.HasNext()
+
+requires c in l.Iterators() && c.Valid() && c.Parent()==l
+requires 0<=c.Index()<|l.Model()| && 0<=n<=|l.Model()| && c.Index()+n<=|l.Model()|
+requires c.Index()<=p.Index()<c.Index()+n && c.Index()<=q.Index()<c.Index()+n
+
+
+
+ensures l.Valid() && p.Valid() && q.Valid()
+ensures p.Parent()==l && q.Parent()==l
+
+ensures |l.Model()|==|old(l.Model())|
+ensures l.Model()[old(q.Index())] == old(l.Model())[old(p.Index())]
+ensures l.Model()[old(p.Index())] == old(l.Model())[old(q.Index())]
+ensures forall i | 0<=i<|l.Model()| && i!=old(p.Index()) && i != old(q.Index()) :: l.Model()[i]==old(l.Model())[i]
+ensures multiset(l.Model())==multiset(old(l.Model()))
+
+ensures l.Iterators()>=old(l.Iterators())
+ensures p in l.Iterators() && q in l.Iterators() && p.Index()==old(p.Index()) && q.Index()==old(q.Index())
+ensures forall it | it in old(l.Iterators()) && old(it.Valid())::it.Valid() && it.Index()==old(it.Index())
+
+ensures forall x {:trigger x in l.Repr(), x in old(l.Repr())} | x in l.Repr() && x !in old(l.Repr()) :: fresh(x)
+ensures fresh(l.Repr()-old(l.Repr()))
+ensures forall x | x in l.Repr() :: allocated(x)
+
+//ADDITIONAL GHOST INFO
+ensures c in l.Iterators() && c.Valid() && c.Parent()==l && c.Index()==old(c.Index())
+ensures |l.Model()|==|old(l.Model())| && 0<=c.Index()<=c.Index()+n<=|l.Model()|
+ensures multiset(l.Model()[c.Index()..c.Index()+n])== multiset(old(l.Model()[c.Index()..c.Index()+n]))
+//ensures l.Model()[..c.Index()] == old(l.Model()[..c.Index()]) && l.Model()[c.Index()+n..] == old(l.Model()[c.Index()+n..]) 
+
+{
+     var auxq :=q.Peek();
+     var auxp:= p.Peek();
+     p.Set(auxq);
+     q.Set(auxp);
+     
+      swapMultiset(l.Model(),old(l.Model()),p.Index(),q.Index());
+      assert 0<=c.Index()<=c.Index()+n<=|l.Model()|;
+      swapMultiset(l.Model()[c.Index()..c.Index()+n],old(l.Model()[c.Index()..c.Index()+n]),p.Index()-c.Index(),q.Index()-c.Index());
+     
+}
+
+
+
+method  {:verify false} partitionG(l:LinkedList,c:ListIterator,n:int, x:int) returns (p:ListIterator,nL:int,q:ListIterator,nG:int)
+modifies l, l.Repr()
+requires l.Valid() && c.Valid() 
+requires c.Parent()==l && c in l.Iterators() 
+requires 0<=n<= |l.Model()| && 0<=c.Index()<=c.Index()+n<=|l.Model()|
+requires forall x | x in l.Repr() :: allocated(x)
+
+ensures l.Valid()
+ensures p.Valid() && q.Valid()
+ensures p.Parent()==l && q.Parent()==l && c.Parent()==l 
+ensures c.Valid() && c.Index()==old(c.Index()) 
+ensures 0<=c.Index()<=p.Index()<=q.Index()<=c.Index()+n<=|l.Model()|
+ensures |l.Model()|==|old(l.Model())|
+
+ensures l.Iterators() >= {p,q}+old(l.Iterators())
+ensures forall it | it in old(l.Iterators()) && old(it.Valid()) :: it.Valid() && it.Index()==old(it.Index())
+
+
+ensures multiset(l.Model()[c.Index()..c.Index()+n])== multiset(old(l.Model()[c.Index()..c.Index()+n]))
+ensures l.Model()[..c.Index()] == old(l.Model()[..c.Index()]) && l.Model()[c.Index()+n..] == old(l.Model()[c.Index()+n..]) 
+ensures forall z | c.Index()<=z<p.Index() :: l.Model()[z]<x
+ensures forall z | p.Index()<=z<q.Index() :: l.Model()[z]==x
+ensures forall z | q.Index()<=z<c.Index()+n:: l.Model()[z]>x
+ensures nL==p.Index()-c.Index() && nG == c.Index()+n-q.Index()
+ensures x in multiset(old(l.Model()[c.Index()..c.Index()+n])) ==> p.Index()<q.Index()
+
+ensures forall x {:trigger x in l.Repr(), x in old(l.Repr())} | x in l.Repr() && x !in old(l.Repr()) :: fresh(x)
+ensures fresh(l.Repr()-old(l.Repr()))
+ensures forall x | x in l.Repr() :: allocated(x)
+{
+  var aux;
+  p:=c.Copy();
+  q:=c.Copy();
+  var r:=c.Copy();
+
+   var i:=0;nL:=0;nG:=0;
+
+   while (i<n)
+    decreases n-i
+    invariant 0<=i<=n
+    invariant l.Valid() && c.Valid() && c.Parent()==l 
+    invariant p.Valid() && q.Valid() && r.Valid()
+    invariant p.Parent()==l && q.Parent()==l && r.Parent()==l
+    invariant r.Index()==c.Index()+i && c.Index()<=p.Index()<=q.Index()<=r.Index()<=c.Index()+n<=|l.Model()|
+    invariant |l.Model()|==|old(l.Model())|
+    invariant  multiset(l.Model())==multiset(old(l.Model()))
+    invariant nL==p.Index()-c.Index() && nG == r.Index()-q.Index()
+    invariant x in multiset(l.Model()[c.Index()..r.Index()]) ==> p.Index()<q.Index()
+    
+    invariant forall z | c.Index()<=z<p.Index() :: l.Model()[z]<x
+    invariant forall z | p.Index()<=z<q.Index() :: l.Model()[z]==x
+    invariant forall z | q.Index()<=z<r.Index() :: l.Model()[z]>x
+
+    invariant multiset(l.Model()[c.Index()..c.Index()+n])== multiset(old(l.Model()[c.Index()..c.Index()+n]))
+    invariant l.Model()[..c.Index()] == old(l.Model()[..c.Index()]) && l.Model()[c.Index()+n..] == old(l.Model()[c.Index()+n..]) 
+
+    invariant l.Iterators() >= {p,q,r}+old(l.Iterators())
+    invariant forall it | it in old(l.Iterators()) && old(it.Valid()) :: it.Valid() && it.Index()==old(it.Index())
+
+
+    invariant forall x {:trigger x in l.Repr(), x in old(l.Repr())} | x in l.Repr() && x !in old(l.Repr()) :: fresh(x)
+    invariant fresh(l.Repr()-old(l.Repr()))
+    invariant forall x | x in l.Repr() :: allocated(x)
+  {
+   if (r.Peek()>x)
+    {  nG:=nG+1; }
+   else if (r.Peek()==x)
+    { 
+     swapG(l,q,r,c,n);
+     aux:=q.Next();
+    }  
+   else {
+   
+     swapG(l,q,r,c,n);
+     swapG(l,p,q,c,n);
+     aux:=p.Next();
+     aux:=q.Next();
+     nL:=nL+1;
+     
+  }
+  aux:= r.Next();
+  i:=i+1;
+    
+}
+assert r.Index()==c.Index()+n;
+
+}
+
+method {:verify true} {:timeLimitMultiplier 6} quicksort(l:LinkedList,c:ListIterator,n:int)
+decreases n
+modifies l, l.Repr()
+requires l.Valid() && c in l.Iterators() && c.Valid() && c.Parent()==l 
+requires forall x | x in l.Repr() :: allocated(x)
+requires 0<=c.Index()<=|l.Model()| && 0<=n<=|l.Model()| && c.Index()+n<=|l.Model()|
+
+ensures l.Valid() && c in l.Iterators() && c.Valid() && c.Parent()==l 
+ensures c.Valid() &&  c.Index()==old(c.Index()) && 0<=c.Index()<=c.Index()+n<=|l.Model()|
+
+ensures multiset(l.Model()[c.Index()..c.Index()+n])== multiset(old(l.Model())[c.Index()..c.Index()+n])
+ensures GSorted(l.Model(),c.Index(),c.Index()+n)
+ensures l.Model()[..c.Index()] == old(l.Model()[..c.Index()]) && l.Model()[c.Index()+n..] == old(l.Model()[c.Index()+n..]) 
+
+
+ensures l.Iterators() >= old(l.Iterators())
+ensures forall it | it in old(l.Iterators()) && old(it.Valid()) ::it.Valid() && it.Index()==old(it.Index())
+
+ensures forall x {:trigger x in l.Repr(), x in old(l.Repr())} | x in l.Repr() && x !in old(l.Repr()) :: fresh(x)
+ensures fresh(l.Repr()-old(l.Repr()))
+ensures forall x | x in l.Repr() :: allocated(x)
+{
+  var p,q:ListIterator;var nL,nG:int;
+  if (n>1)
+  {
+      var omodel:=l.Model();
+   
+   p,nL,q,nG:=partitionG(l,c,n,c.Peek());
+     
+      assert q.Index()+nG==c.Index()+n;
+   
+      var omodel1:=l.Model();
+      assert multiset(omodel1[c.Index()..c.Index()+n])== multiset(omodel[c.Index()..c.Index()+n]);
+      assert forall z | c.Index()+nL <= z <q.Index() ::omodel1[z]==omodel1[c.Index()+nL];
+
+   
+   quicksort(l,c,nL);
+    
+
+      var omodel2:=l.Model();
+
+      assert multiset(omodel2[c.Index()..c.Index()+nL])== multiset(omodel1[c.Index()..c.Index()+nL]);
+      assert omodel2[..c.Index()] == omodel1[..c.Index()] && omodel2[c.Index()+nL..] == omodel1[c.Index()+nL..]; 
+      
+      seqSplit(omodel2,c.Index(),c.Index()+nL,c.Index()+n-1);
+      
+      assert 0<=c.Index()<=c.Index()+nL<=c.Index()+n<=|omodel1|;
+      seqSplit(omodel1,c.Index(),c.Index()+nL,c.Index()+n-1);
+    
+      calc =={
+        multiset(omodel2[c.Index()..c.Index()+n]);
+        multiset(omodel2[c.Index()..c.Index()+nL])+multiset(omodel2[c.Index()+nL..c.Index()+n]);
+        {assert omodel2[c.Index()+nL..] == omodel1[c.Index()+nL..];
+        subsecEq(omodel2[c.Index()+nL..],omodel1[c.Index()+nL..],0,n-nL); 
+         assert omodel2[c.Index()+nL..c.Index()+n] == omodel1[c.Index()+nL..c.Index()+n]; }
+        multiset(omodel1[c.Index()..c.Index()+nL])+multiset(omodel1[c.Index()+nL..c.Index()+n]);
+        multiset(omodel1[c.Index()..c.Index()+n]);
+      }
+   
+
+       multisetPreservesStrictSmaller(omodel1,omodel2,c.Index(),c.Index()+nL-1,omodel2[c.Index()+nL]);
+       assert GSorted(omodel2,c.Index(),c.Index()+nL);
+       assert forall z | c.Index()+nL <= z <q.Index() ::omodel2[z]==omodel2[c.Index()+nL];
+
+    quicksort(l,q,nG);
+    
+      assert multiset(l.Model()[q.Index()..q.Index()+nG])== multiset(omodel2[q.Index()..q.Index()+nG]);
+      assert l.Model()[..q.Index()] == omodel2[..q.Index()] && l.Model()[q.Index()+nG..] == omodel2[q.Index()+nG..]; 
+      assert c.Index()+nL<=q.Index();
+      seqSplit(l.Model(),c.Index(),q.Index(),c.Index()+n-1);
+      seqSplit(omodel2,c.Index(),q.Index(),c.Index()+n-1);
+      calc =={
+        multiset(l.Model()[c.Index()..c.Index()+n]);
+        multiset(l.Model()[c.Index()..q.Index()])+multiset(l.Model()[q.Index()..c.Index()+n]);
+        {assert l.Model()[c.Index()..q.Index()] == omodel2[c.Index()..q.Index()]; }
+        multiset(omodel2[c.Index()..q.Index()])+multiset(omodel2[q.Index()..c.Index()+n]);
+        multiset(omodel2[c.Index()..c.Index()+n]);
+      }
+
+      assert multiset(l.Model()[c.Index()..c.Index()+n])== multiset(old(l.Model())[c.Index()..c.Index()+n]);
+
+      multisetPreservesStrictGreater(omodel2,l.Model(),q.Index(),c.Index()+n-1,omodel2[c.Index()+nL]);
+      assert GSorted(l.Model(),q.Index(),c.Index()+n);
+      assert GSorted(l.Model(),c.Index(),c.Index()+nL);
+
+      assert l.Model()[c.Index()+nL..q.Index()]==omodel1[c.Index()+nL..q.Index()];
+      assert forall z | c.Index()<=z<c.Index()+nL :: l.Model()[z]<l.Model()[c.Index()+nL];
+      assert forall z | c.Index()+nL <= z <q.Index() :: l.Model()[z]==l.Model()[c.Index()+nL];
+      assert forall z | q.Index()<=z<c.Index()+n:: l.Model()[z]>l.Model()[c.Index()+nL];
+      assert GSorted(l.Model(),c.Index(),c.Index()+n);
+  }
+}
+
+
+
+
